Flesh out state relation and refine cheats
The state relation is still inadequate for two reasons.

- It needs to state that two differently named globals are stored
  in distinct memory locations.

- It is built on the (reasonable) expectation that if you store
  something and load it back, you get the same value back that you put
  in.  This is only true if the value's size is below 2^dimindex.  In
  practice all values will of course have this property, but there's
  currently not enough information in the state relation to know this.

pancake/proofs/pan_globalsProofScript.sml
@@ -4,10 +4,11 @@
 
 open preamble
      panSemTheory panLangTheory pan_globalsTheory panPropsTheory
+     stack_removeProofTheory (* TODO: just for addresses_def. should this be moved? *)
 
 val _ = new_theory "pan_globalsProof";
 
-val _ = set_grammar_ancestry  ["panSem", "pan_globals", "panProps", "panLang"];
+val _ = set_grammar_ancestry  ["panSem", "pan_globals", "panProps", "panLang", "stack_removeProof"];
 
 val s = ``s:('a,'ffi) panSem$state``
 
@@ -22,7 +23,8 @@ Definition state_rel_def:
   (∀v val.
      FLOOKUP s.globals v = SOME val ⇒
      ∃addr. FLOOKUP ctxt.globals v = SOME(shape_of val, addr) ∧
-            mem_load (shape_of val) (t.top_addr - addr) t.memaddrs t.memory = SOME val
+            mem_load (shape_of val) (t.top_addr - addr) t.memaddrs t.memory = SOME val ∧
+            DISJOINT s.memaddrs (addresses (t.top_addr - addr) $ size_of_shape $ shape_of val)
   ) ∧
   s.memaddrs ⊆ t.memaddrs ∧
   s.sh_memaddrs = t.sh_memaddrs ∧
@@ -169,10 +171,107 @@ Proof
   gvs[state_rel_def]
 QED
 
+(* TODO: move? *)
+Theorem mem_stores_append:
+  ∀addr vs addrs memory vs'.
+    mem_stores addr (vs ++ vs') addrs memory =
+    case mem_stores addr vs addrs memory of
+    NONE => NONE
+    | SOME memory' => mem_stores (addr + bytes_in_word * n2w(LENGTH vs)) vs' addrs memory'
+Proof
+  Induct_on ‘vs’ >>
+  rw[mem_stores_def] >>
+  rpt (TOP_CASE_TAC >> gvs[n2w_SUC,WORD_LEFT_ADD_DISTRIB])
+QED
+
+Theorem mem_stores_memory_swap:
+  ∀addr vs addrs memory memory' m.
+    mem_stores addr vs addrs memory = SOME m ⇒
+    ∃m'. mem_stores addr vs addrs memory' = SOME m'
+Proof
+  Induct_on ‘vs’ >> rw[mem_stores_def,AllCaseEqs(), mem_store_def] >>
+  metis_tac[]
+QED
+
+Theorem mem_load_mem_store:
+  (∀s (addr:'a word) addrs memory v w.
+     mem_load s addr addrs memory = SOME v ∧
+     shape_of w = s ⇒
+     ∃m. mem_stores addr (flatten w) addrs memory = SOME m) ∧
+  (∀ss (addr:'a word) addrs memory vs ws.
+     mem_loads ss addr addrs memory = SOME vs ∧
+     ss = MAP shape_of ws ⇒
+     ∃m. mem_stores addr (FLAT (MAP (λa. flatten a) ws)) addrs memory = SOME m)
+Proof
+  ho_match_mp_tac mem_load_ind >>
+  rw[mem_load_def,AllCaseEqs()]
+  >- (gvs[Once $ oneline shape_of_def] >>
+      gvs[AllCaseEqs(),mem_stores_def,flatten_def,mem_store_def])
+  >- (first_x_assum $ drule_then drule >>
+      strip_tac >>
+      gvs[Once $ oneline shape_of_def,AllCaseEqs(),ETA_THM,flatten_def])
+  >- simp[mem_stores_def]
+  >- (gvs[MAP_EQ_CONS |> CONV_RULE $ LHS_CONV SYM_CONV] >>
+      first_x_assum drule >> simp[] >>
+      strip_tac >>
+      simp[mem_stores_append] >>
+      gvs[Once $ oneline shape_of_def, AllCaseEqs(), flatten_def, size_of_shape_def, ETA_THM] >>
+      gvs[mem_stores_def,mem_store_def,AllCaseEqs()] >>
+      metis_tac[mem_stores_memory_swap])
+  >- (gvs[MAP_EQ_CONS |> CONV_RULE $ LHS_CONV SYM_CONV] >>
+      first_x_assum $ resolve_then Any mp_tac EQ_REFL >>
+      strip_tac >>
+      simp[mem_stores_append] >>
+      qpat_x_assum ‘_ = shape_of _’ $ assume_tac o GSYM >>
+      gvs[Once $ oneline shape_of_def, AllCaseEqs(), flatten_def, size_of_shape_def, ETA_THM, LENGTH_FLAT] >>
+      gvs[MAP_MAP_o,o_DEF,length_flatten_eq_size_of_shape] >>
+      metis_tac[mem_stores_memory_swap])
+QED
+
+Theorem mem_stores_mem_load_back:
+  (∀val (addr:'a word) addrs memory m.
+    mem_stores addr (flatten val) addrs memory = SOME m ⇒
+    mem_load (shape_of val) addr addrs m =
+    SOME val) ∧
+  (∀vals (addr:'a word) addrs memory m.
+    mem_stores addr (FLAT (MAP (λa. flatten a) vals)) addrs memory = SOME m ⇒
+    mem_loads (MAP shape_of vals) addr addrs m =
+    SOME vals)
+Proof
+  ho_match_mp_tac v_induction >>
+  rw[flatten_def,shape_of_def,mem_stores_def,AllCaseEqs(),
+     mem_store_def,mem_load_def
+    ] >>
+  rw[UPDATE_APPLY]
+  >- (rw[Once $ oneline shape_of_def] >> PURE_CASE_TAC >> simp[])
+  >- metis_tac[]
+  >- (gvs[mem_stores_append,AllCaseEqs()] >>
+      res_tac >>
+      fs[] >>
+      gvs[] >>
+
+
+     )
+     )
+  >- ()
+
+QED
+
 Theorem compile_Assign_Global:
   ^(get_goal "compile _ (Assign Global _ _)")
 Proof
-  cheat
+  rw[evaluate_def,compile_def,AllCaseEqs(),
+     is_valid_value_def,good_res_def
+    ] >>
+  drule_all_then strip_assume_tac compile_exp_correct >>
+  gvs[state_rel_def] >>
+  res_tac >>
+  fs[evaluate_def,eval_def,wordLangTheory.word_op_def] >>
+  drule $ cj 1 mem_load_mem_store >>
+  disch_then drule >>
+  strip_tac >>
+  simp[] >>
+  cheat (* unprovable *)
 QED
 
 Theorem state_rel_res_var[local]:
@@ -198,16 +297,56 @@ Proof
   gvs[state_rel_def]
 QED
 
+Theorem state_rel_memory_update:
+  state_rel T ctxt s t ∧ addr ∈ s.memaddrs ⇒
+  state_rel T ctxt (s with memory := s.memory⦇addr ↦ h⦈) (t with memory := t.memory⦇addr ↦ h⦈)
+Proof
+  rw[] >>
+  gvs[state_rel_def] >>
+  reverse conj_tac >- rw[APPLY_UPDATE_THM] >>
+  rw[] >>
+  res_tac >>
+  first_assum $ irule_at $ Pos hd >>
+  simp[] >>
+  cheat (* provable*)
+QED
+
 Theorem compile_Store:
   ^(get_goal "compile _ (Store _ _)")
 Proof
-  cheat
+  rw[evaluate_def,compile_def,AllCaseEqs(),UNCURRY_eq_pair,SF DNF_ss] >>
+  imp_res_tac compile_exp_correct >>
+  simp[] >>
+  gvs[good_res_def] >>
+  rpt $ qpat_x_assum ‘eval _ _ = _’ kall_tac >>
+  rename1 ‘mem_stores _ v’ >>
+  rpt $ pop_assum mp_tac >>
+  MAP_EVERY qid_spec_tac [‘v’,‘s’,‘t’,‘addr’,‘m’] >>
+  Induct_on ‘v’
+  >- (rw[mem_stores_def] >>
+      ‘s with memory := s.memory = s’ by simp[state_component_equality] >>
+      ‘t with memory := t.memory = t’ by simp[state_component_equality] >>
+      simp[]) >>
+  rw[mem_stores_def,AllCaseEqs(),mem_store_def] >>
+  ‘addr ∈ t.memaddrs’ by(gvs[state_rel_def,SUBSET_DEF]) >>
+  simp[] >>
+  drule_all state_rel_memory_update >>
+  strip_tac >>
+  first_x_assum (fn thm => first_x_assum $ resolve_then Any mp_tac thm) >>
+  simp[]
 QED
 
 Theorem compile_StoreByte:
   ^(get_goal "compile _ (StoreByte _ _)")
 Proof
-  cheat
+  rw[evaluate_def,compile_def,AllCaseEqs(),UNCURRY_eq_pair,SF DNF_ss, mem_store_byte_def,
+     good_res_def] >>
+  imp_res_tac compile_exp_correct >>
+  ‘s.be = t.be’ by gvs[state_rel_def] >>
+  simp[] >>
+  irule_at (Pos last) state_rel_memory_update >>
+  simp[] >>
+  gvs[state_rel_def,SUBSET_DEF]
 QED
 
 Triviality v_neq_v':
@@ -231,7 +370,8 @@ Proof
       drule_all_then strip_assume_tac compile_exp_correct >>
       rename1 ‘FLOOKUP _ _ = SOME(Val vv)’ >>
       ‘∃addr. FLOOKUP ctxt.globals v = SOME(shape_of(Val vv), addr) ∧
-              mem_load (shape_of(Val vv)) (t.top_addr - addr) t.memaddrs t.memory = SOME(Val vv)’
+              mem_load (shape_of(Val vv)) (t.top_addr - addr) t.memaddrs t.memory = SOME(Val vv) ∧
+              DISJOINT s.memaddrs (addresses (t.top_addr - addr) (size_of_shape(shape_of(Val vv))))’
         by gvs[state_rel_def] >>
       ‘s.locals = t.locals’ by gvs[state_rel_def] >>
       ‘s.sh_memaddrs = t.sh_memaddrs’ by gvs[state_rel_def] >>
@@ -244,10 +384,34 @@ Proof
           lookup_kvar_def,sh_mem_load_def,AllCaseEqs(),
           wordLangTheory.word_op_def,set_kvar_def,set_var_def,set_global_def,
           mem_stores_def,mem_store_def,mem_load_def,flatten_def]
-      >- cheat
+      >- (gvs[state_rel_def,good_res_def] >>
+          conj_tac
+          >- (rw[fmap_eq_flookup,FLOOKUP_pan_res_var_thm,FLOOKUP_UPDATE] >> rw[]) >>
+          conj_tac
+          >- (cheat (* unprovable? *)) >>
+          rw[] >>
+          gvs[SUBSET_DEF] >>
+          res_tac >>
+          gvs[size_of_shape_def,shape_of_def] >>
+          qhdtm_x_assum ‘DISJOINT’ mp_tac >>
+          rw[Once $ oneline addresses_def, addresses_def] >>
+          rw[APPLY_UPDATE_THM] >>
+          gvs[])
       >- (gvs[state_rel_def,empty_locals_def,good_res_def] >>
           rw[fmap_eq_flookup,FLOOKUP_pan_res_var_thm,FLOOKUP_UPDATE])
-      >- cheat
+      >- (gvs[state_rel_def,good_res_def] >>
+          conj_tac
+          >- (rw[fmap_eq_flookup,FLOOKUP_pan_res_var_thm,FLOOKUP_UPDATE] >> rw[]) >>
+          conj_tac
+          >- (cheat (* unprovable? *)) >>
+          rw[] >>
+          gvs[SUBSET_DEF] >>
+          res_tac >>
+          gvs[size_of_shape_def,shape_of_def] >>
+          qhdtm_x_assum ‘DISJOINT’ mp_tac >>
+          rw[Once $ oneline addresses_def, addresses_def] >>
+          rw[APPLY_UPDATE_THM] >>
+          gvs[])
       >- (gvs[state_rel_def,empty_locals_def,good_res_def] >>
           rw[fmap_eq_flookup,FLOOKUP_pan_res_var_thm,FLOOKUP_UPDATE]))
 QED
